## **1. Multiplication Property of Modular Arithmetic**

For integers $A$, $B$, and modulus $C$:

$$
(A \cdot B) \bmod C = (A \bmod C \cdot B \bmod C) \bmod C
$$

---

## **2. Statement to Be Proven**

We prove:

$$
(A \cdot B) \bmod C = (A \bmod C \cdot B \bmod C) \bmod C
$$

The goal is to show **LHS = RHS**.

---

## **3. Representation Using the Quotient Remainder Theorem**

By the quotient remainder theorem, we write:

- $A = C \cdot Q_1 + R_1$, where $0 \le R_1 < C$  
  Hence, $A \bmod C = R_1$

- $B = C \cdot Q_2 + R_2$, where $0 \le R_2 < C$  
  Hence, $B \bmod C = R_2$

---

## **4. Left-Hand Side (LHS)**

$$
\text{LHS} = (A \cdot B) \bmod C
$$

Substitute the expressions for $A$ and $B$:

$$
\text{LHS}
= \big((C \cdot Q_1 + R_1)(C \cdot Q_2 + R_2)\big) \bmod C
$$

Expand the product:

$$
\text{LHS}
= \big(C^2 Q_1 Q_2 + C Q_1 R_2 + C Q_2 R_1 + R_1 R_2\big) \bmod C
$$

Factor out $C$ from the first three terms:

$$
\text{LHS}
= \big(C(C Q_1 Q_2 + Q_1 R_2 + Q_2 R_1) + R_1 R_2\big) \bmod C
$$

Multiples of $C$ vanish under modulo $C$:

$$
\text{LHS} = (R_1 R_2) \bmod C
$$

---

## **5. Right-Hand Side (RHS)**

$$
\text{RHS} = (A \bmod C \cdot B \bmod C) \bmod C
$$

Substitute $A \bmod C = R_1$ and $B \bmod C = R_2$:

$$
\text{RHS} = (R_1 R_2) \bmod C
$$

---

## **6. Conclusion**

Since:

$$
\text{LHS} = (R_1 R_2) \bmod C
$$

and

$$
\text{RHS} = (R_1 R_2) \bmod C
$$

we conclude:

$$
\text{LHS} = \text{RHS}
$$

Therefore, the multiplication property of modular arithmetic holds.
